backend/RTLtypingC.v
@@ -29,110 +29,6 @@ Require Import Conventions.
 Require Import sflib.
 (** newly added **)
 Require Export RTLtyping.
-
-Inductive wt_stackframes: list stackframe -> signature -> Prop :=
-  | wt_stackframes_nil: forall sg,
-      wt_stackframes nil sg
-  | wt_stackframes_cons:
-      forall s res f sp pc rs env sg,
-      wt_function f env ->
-      wt_regset env rs ->
-      env res = proj_sig_res sg ->
-      wt_stackframes s (fn_sig f) ->
-      wt_stackframes (Stackframe res f sp pc rs :: s) sg.
-
-Inductive wt_state: state -> Prop :=
-  | wt_state_intro:
-      forall s f sp pc rs m env
-        (WT_STK: wt_stackframes s (fn_sig f))
-        (WT_FN: wt_function f env)
-        (WT_RS: wt_regset env rs),
-      wt_state (State s f sp pc rs m)
-  | wt_state_call:
-      forall s fptr sg args m,
-      wt_stackframes s sg ->
-      DUMMY_PROP ->
-      Val.has_type_list args (sig_args sg) ->
-      wt_state (Callstate s fptr sg args m)
-  | wt_state_return:
-      forall s v m sg,
-      wt_stackframes s sg ->
-      Val.has_type v (proj_sig_res sg) ->
-      wt_state (Returnstate s v m).
-
-Remark wt_stackframes_change_sig:
-  forall s sg1 sg2,
-  sg1.(sig_res) = sg2.(sig_res) -> wt_stackframes s sg1 -> wt_stackframes s sg2.
-Proof.
-  intros. inv H0.
-- constructor; congruence.
-- econstructor; eauto. rewrite H3. unfold proj_sig_res. rewrite H. auto.
-Qed.
-
-Section SUBJECT_REDUCTION.
-
-Variable p: program.
-
-Hypothesis wt_p: wt_program p.
-
-Variable se: Senv.t.
-Variable ge: genv.
-
-Hypothesis CONTAINED: forall
-    fptr f
-    (FINDF: Genv.find_funct ge fptr = Some f)
-  ,
-    exists i, In (i, Gfun f) (prog_defs p)
-.
-
-Lemma subject_reduction:
-  forall st1 t st2, step se ge st1 t st2 ->
-  forall (WT: wt_state st1), wt_state st2.
-Proof.
-  induction 1; intros; inv WT;
-  try (generalize (wt_instrs _ _ WT_FN pc _ H); intros WTI).
-  (* Inop *)
-  econstructor; eauto.
-  (* Iop *)
-  econstructor; eauto. eapply wt_exec_Iop; eauto.
-  (* Iload *)
-  econstructor; eauto. eapply wt_exec_Iload; eauto.
-  (* Istore *)
-  econstructor; eauto.
-  (* Icall *)
-  econstructor; eauto.
-  econstructor; eauto. inv WTI; auto.
-  inv WTI. rewrite <- H8. apply wt_regset_list. auto.
-  (* Itailcall *)
-  econstructor; eauto.
-  inv WTI. apply wt_stackframes_change_sig with (fn_sig f); auto.
-  inv WTI. rewrite <- H7. apply wt_regset_list. auto.
-  (* Ibuiltin *)
-  econstructor; eauto. eapply wt_exec_Ibuiltin; eauto.
-  (* Icond *)
-  econstructor; eauto.
-  (* Ijumptable *)
-  econstructor; eauto.
-  (* Ireturn *)
-  econstructor; eauto.
-  inv WTI; simpl. auto. unfold proj_sig_res; rewrite H2. auto.
-  (* internal function *)
-  assert(H5: wt_fundef (Internal f)). exploit CONTAINED; eauto. i; des. eapply wt_p; eauto.
-  simpl in *. inv H5.
-  econstructor; eauto.
-  inv H1. apply wt_init_regs; auto. rewrite wt_params. auto.
-  (* external function *)
-  econstructor; eauto. simpl.
-  eapply external_call_well_typed; eauto.
-  (* return *)
-  inv H1. econstructor; eauto.
-  apply wt_regset_assign; auto. rewrite H10; auto.
-Qed.
-
-End SUBJECT_REDUCTION.
-
-
-
 Require Import Skeleton ModSem Preservation.
 Require Import SoundTop.
 Require Import RTLC.
@@ -148,7 +44,7 @@ Section LPRSV.
   Theorem wt_state_local_preservation
           skenv_link
     :
-      local_preservation (modsem skenv_link prog) (fun _ _ st => wt_state st)
+      local_preservation (modsem skenv_link prog) (fun _ _ st => wt_state true st)
   .
   Proof.
     econs; ii; ss; eauto.
